src/arch/x64/X64.Memory_i_s.fsti
@@ -302,6 +302,7 @@ val lemma_valid_store_mem128: i:int -> v:quad32 -> h:mem -> Lemma (
 val bytes_valid (i:int) (s:state) : Lemma
   (requires valid_mem64 i s.mem)
   (ensures S.valid_addr64 i s.state.S.mem)
+  [SMTPat (S.valid_addr64 i s.state.S.mem)]
 
 val valid_state_store_mem64: ptr:int -> v:nat64 -> s:state -> Lemma (
   let s' = { state = if valid_mem64 ptr s.mem then S.update_mem ptr v s.state 
@@ -311,11 +312,20 @@ val valid_state_store_mem64: ptr:int -> v:nat64 -> s:state -> Lemma (
 val bytes_valid128 (i:int) (s:state) : Lemma
   (requires valid_mem128 i s.mem)
   (ensures S.valid_addr128 i s.state.S.mem)
+  [SMTPat (S.valid_addr128 i s.state.S.mem)]
 
 val valid_state_store_mem128: ptr:int -> v:quad32 -> s:state -> Lemma (
   let s' = { state = if valid_mem128 ptr s.mem then S.update_mem128 ptr v s.state 
   else s.state; mem = store_mem128 ptr v s.mem } in
   valid_state s')
+
+val equiv_load_mem: ptr:int -> s:state -> Lemma
+  (requires valid_mem64 ptr s.mem)
+  (ensures load_mem64 ptr s.mem == S.eval_mem ptr s.state)
+
+val equiv_load_mem128: ptr:int -> s:state -> Lemma
+  (requires valid_mem128 ptr s.mem)
+  (ensures load_mem128 ptr s.mem == S.eval_mem128 ptr s.state)
 
 //Memtaint related functions
 
