src/arch/x64/X64.Semantics_Equiv_i.fsti
@@ -1,0 +1,20 @@
+module X64.Semantics_Equiv_i
+
+module S = X64.Bytes_Semantics_s
+open X64.Memory_i_s
+open X64.Semantics_s
+
+val equiv_eval_ins (s:state) (ins:S.ins) : Lemma (
+   let s_hi = run (eval_ins ins) s in
+   let s_bytes = S.run (S.eval_ins ins) s.state in
+   s_hi.state.S.ok /\ s_bytes.S.ok ==> s_hi.state == s_bytes)
+
+// val equiv_eval_code (s:state) (fuel:nat) (code:code) : Lemma (
+//   let s_hi = eval_code code fuel s in
+//   let s_bytes = S.eval_code code fuel s.state in
+//     (None? s_hi /\ None? s_bytes) \/
+//   ( Some? s_hi /\ Some? s_bytes /\ 
+//     ((Some?.v s_hi).state.S.ok /\ (Some?.v s_bytes).S.ok ==> 
+//     (Some?.v s_hi).state == Some?.v s_bytes
+//   ))
+// )
